src/program_proof/wal/read_proof.v
@@ -32,16 +32,51 @@ Admitted.
 
 Opaque struct.t.
 
+Theorem memLog_split_combine (s: Slice.t) memStart nextDiskEnd (q: Qp) memLog :
+  Qcanon.Qclt q 1 ->
+    let boundary := (int.nat nextDiskEnd - int.nat memStart)%nat in
+    updates_slice_frag s q (take boundary memLog) ∗
+    updates_slice_frag (slice_skip s (struct.t Update.S) (word.sub nextDiskEnd memStart)) 1
+                        (drop boundary memLog)
+                        ⊣⊢
+    updates_slice_frag s (q/2) memLog ∗
+    (updates_slice_frag s (q/2) memLog ∗
+      ∃ q',⌜(1-q/2)%Qp=Some q'⌝ ∗ updates_slice_frag (slice_skip s (struct.t Update.S) (word.sub nextDiskEnd memStart)) q'
+                      (drop boundary memLog)).
+Proof.
+Admitted.
+
+Theorem memLog_combine (s: Slice.t) memStart nextDiskEnd (q: Qp) memLog :
+  Qcanon.Qclt q 1 ->
+    let boundary := (int.nat nextDiskEnd - int.nat memStart)%nat in
+    updates_slice_frag s q (take boundary memLog) ∗
+    updates_slice_frag (slice_skip s (struct.t Update.S) (word.sub nextDiskEnd memStart)) 1
+                        (drop boundary memLog) -∗
+                        updates_slice_frag s (q/2) memLog ∗
+   (updates_slice_frag s (q/2) memLog -∗
+     (* could drop this conjunct (it doesn't need to go back
+     into the [readonly]) *)
+     updates_slice_frag s q (take boundary memLog) ∗
+     updates_slice_frag (slice_skip s (struct.t Update.S) (word.sub nextDiskEnd memStart)) 1
+                        (drop boundary memLog)).
+Proof.
+  intros.
+  rewrite memLog_split_combine; auto.
+  iIntros "(Hfrag1&Hfrag2&Habsorb)".
+  iFrame.
+  auto.
+Qed.
+
 Theorem wp_WalogState__readMem γ (st: loc) σ (a: u64) :
   {{{ wal_linv_fields st σ ∗
-      memLog_linv γ σ.(memStart) σ.(memLog) }}}
+      memLog_linv γ σ.(memStart) σ.(nextDiskEnd) σ.(memLog) }}}
     WalogState__readMem #st #a
   {{{ b_s (ok:bool), RET (slice_val b_s, #ok);
       (if ok then ∃ b, is_block b_s 1 b ∗
                        ⌜apply_upds σ.(memLog) ∅ !! int.val a = Some b⌝
       else ⌜b_s = Slice.nil ∧ apply_upds σ.(memLog) ∅ !! int.val a = None⌝) ∗
       "Hfields" ∷ wal_linv_fields st σ ∗
-      "HmemLog_linv" ∷ memLog_linv γ σ.(memStart) σ.(memLog)
+      "HmemLog_linv" ∷ memLog_linv γ σ.(memStart) σ.(nextDiskEnd) σ.(memLog)
   }}}.
 Proof.
   iIntros (Φ) "(Hfields&HmemLog_inv) HΦ".
@@ -57,12 +92,15 @@ Proof.
     wp_loadField. wp_loadField.
     apply memLogMap_ok_memLog_lookup in Hmapget as [b HmemLog_lookup];
       last by admit. (* TODO: in-bounds proof *)
-    wp_apply (wp_SliceGet_updates with "[$His_memLog]"); eauto.
+    iMod (readonly_load_lt with "His_memLog") as (q) "[%Hqbound HmemLog_slice]"; first by auto.
+    iDestruct (memLog_combine with "[$HmemLog_slice $HabsorbLog]") as "[HmemLog_slice HabsorbLog']"; first by auto.
+    wp_apply (wp_SliceGet_updates with "[$HmemLog_slice]"); eauto.
     simpl.
-    iIntros ([a' u_s]) "(<-&Hb&His_memLog)".
+    iIntros ([a' u_s]) "(<-&Hb&HmemLog_slice)".
     wp_apply (wp_copyUpdateBlock with "Hb").
     iIntros (s') "[Hb Hb_new]".
-    iSpecialize ("His_memLog" with "Hb").
+    iSpecialize ("HmemLog_slice" with "Hb").
+    iDestruct ("HabsorbLog'" with "HmemLog_slice") as "[HmemLog_slice HabsorbLog]".
     wp_pures.
     iApply "HΦ".
     iFrame.
@@ -74,11 +112,11 @@ Proof.
     apply_upds formulation is actually a good way to phrase it, especially since
     [apply_upds] and [compute_memLogMap] are similar fold_left's) *)
       admit.
-    + iExists _; by iFrame.
+    + iExists _; by iFrame "# ∗".
   - wp_pures.
     iApply ("HΦ" $! Slice.nil false).
     iFrame.
-    iSplit; [ | by iExists _; iFrame ].
+    iSplit; [ | iExists _; by iFrame "# ∗" ].
     iPureIntro.
     split; auto.
     (* TODO: need a theorem about missing in compute_memLogMap (should follow
@@ -86,29 +124,29 @@ Proof.
     admit.
 Admitted.
 
-Theorem simulate_read_cache_hit {l γ Q σ memStart memLog b a} :
+Theorem simulate_read_cache_hit {l γ Q σ memStart nextDiskEnd memLog b a} :
   apply_upds memLog ∅ !! int.val a = Some b ->
   (is_wal_inner l γ σ ∗ P σ) -∗
-  memLog_linv γ memStart memLog -∗
+  memLog_linv γ memStart nextDiskEnd memLog -∗
   (∀ (σ σ' : log_state.t) mb,
       ⌜wal_wf σ⌝
         -∗ ⌜relation.denote (log_read_cache a) σ σ' mb⌝ -∗ P σ ={⊤ ∖ ↑N}=∗ P σ' ∗ Q mb) -∗
   |={⊤ ∖ ↑N}=> (is_wal_inner l γ σ ∗ P σ) ∗
               "HQ" ∷ Q (Some b) ∗
-              "HmemLog_linv" ∷ memLog_linv γ memStart memLog.
+              "HmemLog_linv" ∷ memLog_linv γ memStart nextDiskEnd memLog.
 Proof.
 Admitted.
 
-Theorem simulate_read_cache_miss {l γ Q σ memStart memLog a} :
+Theorem simulate_read_cache_miss {l γ Q σ memStart nextDiskEnd memLog a} :
   apply_upds memLog ∅ !! int.val a = None ->
   (is_wal_inner l γ σ ∗ P σ) -∗
-  memLog_linv γ memStart memLog -∗
+  memLog_linv γ memStart nextDiskEnd memLog -∗
   (∀ (σ σ' : log_state.t) mb,
       ⌜wal_wf σ⌝
         -∗ ⌜relation.denote (log_read_cache a) σ σ' mb⌝ -∗ P σ ={⊤ ∖ ↑N}=∗ P σ' ∗ Q mb) -∗
   |={⊤ ∖ ↑N}=> (∃ σ', is_wal_inner l γ σ' ∗ P σ') ∗
               "HQ" ∷ Q None ∗
-              "HmemLog_linv" ∷ memLog_linv γ memStart memLog.
+              "HmemLog_linv" ∷ memLog_linv γ memStart nextDiskEnd memLog.
 Proof.
 Admitted.
 
@@ -146,7 +184,7 @@ Proof.
     { iNext.
       iExists _; iFrame. }
     wp_loadField.
-    wp_apply (release_spec with "[$lk $Hlocked HmemLog_linv Hfields HnextDiskEnd_txn]").
+    wp_apply (release_spec with "[$lk $Hlocked HmemLog_linv Hfields]").
     { iExists _; iFrame "HdiskEnd_at_least Hstart_at_least ∗". }
     wp_pures.
     iApply "HΦ".
@@ -157,7 +195,7 @@ Proof.
     iModIntro.
     iFrame "Hinv".
     wp_loadField.
-    wp_apply (release_spec with "[$lk $Hlocked HmemLog_linv Hfields HnextDiskEnd_txn]").
+    wp_apply (release_spec with "[$lk $Hlocked HmemLog_linv Hfields]").
     { iExists _; iFrame "HdiskEnd_at_least Hstart_at_least ∗". }
     wp_pures.
     iApply "HΦ".
